compute_degree_le

src/tactic/compute_degree.lean
@@ -37,7 +37,7 @@ open tactic interactive expr
 namespace tactic.interactive
 setup_tactic_parser
 
-/--  Given an expression `e`, assuming it is a polyomial, `extract_deg_one_term e` tries to guess
+/--  Given an expression `e`, assuming it is a polyomial, `extract_deg_single_term e` tries to guess
 the `nat_degree` of `e`.  Currently, it supports:
 * `monomial n r`, guessing `n`,
 * `C a`, guessing `0`,
@@ -45,9 +45,9 @@ the `nat_degree` of `e`.  Currently, it supports:
 * `X ^ n`, guessing `n`,
 * everything else, guessing `e.nat_degree`.
 
-The expectation is that the argument of `extract_deg_one_term` is a factor of a summand of an
+The expectation is that the argument of `extract_deg_single_term` is a factor of a summand of an
 expression in a polynomial ring. -/
-meta def extract_deg_one_term : expr → tactic expr
+meta def extract_deg_single_term : expr → tactic expr
 | `(polynomial.X) := to_expr ``(1)
 | e := match e.app_fn with
   | `(coe_fn $ polynomial.monomial %%n) := return n
@@ -57,28 +57,41 @@ meta def extract_deg_one_term : expr → tactic expr
            return $ expr.mk_app val [e]
   end
 
-/--  `extract_deg_one_summand e` takes apart "factors" in the expression `e` and returns them
-as sums of their "guessed degrees", via `extract_deg_one_term`.  When applied to an expression
+/--  `extract_deg_single_summand e` takes apart "factors" in the expression `e` and returns them
+as sums of their "guessed degrees", via `extract_deg_single_term`.  When applied to an expression
 that is a summand in a polynomial, it should correctly guess its `nat_degree`. -/
-meta def extract_deg_one_summand : expr → tactic expr
+meta def extract_deg_single_summand : expr → tactic expr
 | `(has_mul.mul %%a %%b) := do
-                              ga ← extract_deg_one_summand a,
-                              gb ← extract_deg_one_summand b,
+                              ga ← extract_deg_single_summand a,
+                              gb ← extract_deg_single_summand b,
                               mk_app `has_add.add [ga, gb] >>= return
-| e := extract_deg_one_term e >>= return
+| e := extract_deg_single_term e >>= return
 
-/-- `extract_sorted_list_terms_and_degs e` takes an expression `e` looks for summands in `e`
-(assuming the Type of `e` is `R[X]`), and produces a list of pairs `(e',deg)`, where each `e'` is
-a summand of `e` and each `deg` is the "guessed degree" of `e'`.  The list is sorted by increasing
-values of `deg`. -/
-meta def extract_sorted_list_terms_and_degs (e : expr) : tactic (list (expr × ℕ)) :=
+/-- `extract_top_degree_term_and_deg e` takes an expression `e` looks for summands in `e`
+(assuming the Type of `e` is `R[X]`), and produces the pairs `(e',deg)`, where `e'` is
+a summand of `e` of maximal guessed degree equal to `deg`.
+
+The tactic fails if `e` contains no summand (this probably means something else went wrong
+somewhere else). -/
+meta def extract_top_degree_term_and_deg (e : expr) : tactic (expr × ℕ) :=
 let summ := get_summands e in
-do nat_degs ← summ.mmap extract_deg_one_summand,
+do nat_degs ← summ.mmap extract_deg_single_summand,
   eval_nat_degs ← nat_degs.mmap (eval_expr ℕ) <|>
     tactic.fail "Only closed naturals are supported in exponents\n\n",
   let summ_and_degs := summ.zip eval_nat_degs in
-  --  a little wasteful: we sort the list, but then only use the last entry in `compute_degree`
-  return $ summ_and_degs.merge_sort (λ e f : expr × ℕ, e.2 ≤ f.2)
+  match summ_and_degs.argmax (λ e : expr × ℕ, e.2) with
+  | none := tactic.fail
+      "'`compute_degree`' could not find summands: something has gone very wrong!\n\n"
+  | (some first) := return first
+  end
+
+/-  `extract_top_degree_term_and_deg e` returns the first element of
+`extract_sorted_list_terms_and_degs e` and fails if the relevant list is empty.
+meta def extract_top_degree_term_and_deg (e : expr) : tactic (expr × ℕ) :=
+do (first :: _) ← extract_sorted_list_terms_and_degs e |
+  tactic.fail "'`compute_degree`' could not find summands: something has gone very wrong!\n\n",
+return first
+ -/
 
 /--  These are the cases in which an easy lemma computes the degree. -/
 meta def single_term_suggestions : tactic unit :=
@@ -86,6 +99,29 @@ do `[ exact nat_degree_X_pow _ ] *> trace "Try this: exact nat_degree_X_pow _" <
    `[ exact nat_degree_C _ ]     *> trace "Try this: exact nat_degree_C _"     <|>
    `[ exact nat_degree_X ]       *> trace "Try this: exact nat_degree_X"       <|>
    fail "easy lemmas do not work"
+
+/--  `compute_degree_le` tries to solve a goal of the form `f.nat_degree ≤ d`, where `d : ℕ` and `f`
+satisfies:
+* `f` is a sum of expression of the form
+  `C a * X ^ n, C a * X, C a, X ^ n, X, monomial n a, monomial n a * monomial m b`,
+* all exponents and the `n` in `monomial n a` are *closed* terms of type `ℕ`.
+
+If the given degree is smaller than the one that the tactic computes,
+then the tactic suggests the degree that it computed.
+
+The tactic also reports when it is used with non-closed natural numbers as exponents. -/
+meta def compute_degree_le : tactic unit :=
+`[repeat { refine (polynomial.nat_degree_add_le_of rfl.le _ _ _).mpr _ },
+  repeat { rw polynomial.monomial_mul_monomial },
+  try { any_goals { refine polynomial.nat_degree_monomial_le _ _  } },
+  try { any_goals { refine (polynomial.nat_degree_C_mul_le _ _).trans _ } },
+  try { any_goals { norm_num } },
+  all_goals { refl } ] <|>
+do `(polynomial.nat_degree %%tl ≤ %%tr) ← target,
+  (lead,m') ← extract_top_degree_term_and_deg tl,
+  td ← eval_expr ℕ tr,
+  if td < m' then tactic.fail format!"should the degree bound be '{m'}'?\n\n" else
+  tactic.fail "sorry, the tactic failed."
 
 /--  `compute_degree` tries to solve a goal of the form `f.nat_degree = d`, where `d : ℕ` and `f`
 satisfies:
@@ -95,32 +131,21 @@ satisfies:
 * the term with largest exponent is `X ^ n` and is the unique term of its degree (repetitions are
   allowed in terms of smaller degree).
 
-If the given degree does not match what the tactic computes, the tactic suggests the degree it
-computed.
+If the given degree does not match what the tactic computes,
+then the tactic suggests the degree that it computed.
 
-The tactic also reports when it is used with non-closed natural numbers as exponents.
- -/
+The tactic also reports when it is used with non-closed natural numbers as exponents. -/
 meta def compute_degree : tactic unit :=
 single_term_suggestions <|>
 do `(polynomial.nat_degree %%tl = %%tr) ← target,
-  szd ← extract_sorted_list_terms_and_degs tl,
-  match szd.last' with
-  | none := tactic.fail
-    "'`compute_degree`' could not find summands: something has gone very wrong!\n\n"
-  | some (lead, m') := do
-    td ← eval_expr ℕ tr,
-    if m' ≠ td then do tactic.fail format!"should the degree be '{m'}'?\n\n" else
-    do let ffil : list (bool × pexpr) := [(ff, pexpr.of_expr lead)],
-    move_add_with_errors [(ff, pexpr.of_expr lead)] none,
-    `[rw [polynomial.nat_degree_add_eq_right_of_nat_degree_lt, polynomial.nat_degree_X_pow],
-      rw [polynomial.nat_degree_X_pow],
-      refine nat.lt_succ_of_le _,
-      repeat { refine (polynomial.nat_degree_add_le_of rfl.le _ _ _).mpr _ },
-      repeat { rw polynomial.monomial_mul_monomial },
-      try { any_goals { refine polynomial.nat_degree_monomial_le _ _  } },
-      try { any_goals { refine (polynomial.nat_degree_C_mul_le _ _).trans _ } },
-      try { any_goals { norm_num } }
-     ]
-  end
+  (lead,m') ← extract_top_degree_term_and_deg tl,
+  td ← eval_expr ℕ tr,
+  if m' ≠ td then tactic.fail format!"should the degree be '{m'}'?\n\n" else
+  move_add_with_errors [(ff, pexpr.of_expr lead)] none,
+  `[rw [polynomial.nat_degree_add_eq_right_of_nat_degree_lt, polynomial.nat_degree_X_pow],
+    rw [polynomial.nat_degree_X_pow],
+    refine nat.lt_succ_of_le _ ],
+  compute_degree_le
+
 
 end tactic.interactive
